Sal/ConditionedMRDTs/MRDT_Instances/MRDT_Instances.lean
@@ -1,4 +1,5 @@
 import Sal.ConditionedMRDTs.Metatheory.GC_Safety
+import Sal.ConditionedMRDTs.Metatheory.VirtualLCA_Spot
 import Sal.ConditionedMRDTs.MRDT_Instances.GSet.GSet
 import Sal.ConditionedMRDTs.MRDT_Instances.Counter.Counter
 import Sal.ConditionedMRDTs.MRDT_Instances.ORSet.ORSet
